semantics for ops

Is0/Basic.lean
@@ -128,45 +128,81 @@ inductive Op : IsNondet → Type where
   | Isz : Variable Felt → Op InNondet
   | Inv : Variable Felt → Op InNondet
 
--- inductive Det :=
---   | If : Variable Felt → Det → Det
---   | Sequence : Det → Det → Det
---   | SetInput : ℕ → Variable Felt → Variable Felt → Det -- idx -> buffer -> varName -> Det; buffer[idx] := varName
---   | SetOuput : ℕ → Variable Felt → Variable Felt → Det -- idx -> buffer -> varName -> Det; buffer[idx] := varName
---   | Assign : String → DetOp → Det
+open Op
 
--- An MLIR program in the `cirgen` (circuit generation) dialect. MLIR ops that
--- are not pure functions are implemented here, so they can mess with state. 
+instance {x : IsNondet} : HSub (Variable Felt) (Variable Felt) (Op x) := ⟨Op.Sub⟩
+instance {x : IsNondet} : HMul (Variable Felt) (Variable Felt) (Op x) := ⟨Op.Mul⟩
+
+-- Notation for Ops.
+namespace MLIRNotation
+
+scoped prefix:max "C" => Op.Const
+scoped notation:max "⊤" => Op.True
+scoped notation:max "input[" n "]" => Op.GetInput n 0
+scoped notation:max "output[" n "]" => Op.GetOutput n 0
+scoped infix:55 " &₀ " => Op.AndEqz
+scoped notation:55 " guard " c " & " x " with " y:55 => Op.AndCond x c y
+scoped prefix:57 "??₀" => Op.Isz
+scoped prefix:max "Inv" => Op.Inv
+
+end MLIRNotation
+
+-- Evaluate a pure functional circuit operation to get some kind of literal.
+def Op.eval {x} (state : State) (op : Op x) : Lit :=
+  match op with
+  | Const x => .Val x
+  | True => .Constraint (_root_.True)
+  | GetInput i _ => .Val <| state.input.getD i (-42)
+  | GetOutput i _ => .Val <| state.output.getD i (-42)
+  | Sub x y => .Val $ match state.felts x.name, state.felts y.name with
+                        | some x, some y => x - y
+                        | _      , _       => 42
+  | Mul x y => .Val $ match state.felts x.name, state.felts y.name with
+                        | some x, some y => x * y
+                        | _      , _       => 42
+  | AndEqz c x => .Constraint $ match state.props c.name, state.felts x.name with
+                    | some c, some x => c ∧ x = 0
+                    | _      , _     => 42 = 42
+  | AndCond old cond inner =>
+      .Constraint $ match state.props old.name, state.felts cond.name, state.props inner.name with
+        | .some old, .some cond, .some inner => if cond == 0 then old else old ∧ inner
+        | _        , _         , _           => 42 = 42
+  | Isz x => .Val $ match state.felts x.name with
+               | some x => if x == 0 then 1 else 0
+               | _      => 42
+  | Inv x => .Val $ match state.felts x.name with
+               | some x => if x == 0 then 0 else x⁻¹
+               | _      => 42
+
+notation:61 "Γ " st:max " ⟦" p:49 "⟧ₑ" => Op.eval st p
+
 inductive MLIR : IsNondet → Type where
-  | If : Variable Felt → MLIR x → MLIR x
-  | Eqz : Variable Felt → MLIR x
   | Assign : String → Op x → MLIR x
-  | Sequence : MLIR x → MLIR x → MLIR x
+  | Eqz : Variable Felt → MLIR x
+  | If : Variable Felt → MLIR x → MLIR x
   | Nondet : MLIR InNondet → MLIR NotInNondet
+  | Sequence : MLIR x → MLIR x → MLIR x
+  | SetOutput : Variable Felt → Op x → MLIR InNondet
+
+-- Notation for MLIR programs.  
+namespace MLIRNotation
+
+scoped infix:51 "←ₐ " => MLIR.Assign
+scoped prefix:52 "?₀" => MLIR.Eqz
+scoped notation:51 "guard " c " then " x:51 => MLIR.If c x
+scoped prefix:max "nondet" => MLIR.Nondet
+scoped infixr:50 "; " => MLIR.Sequence
+scoped notation:51 (priority := high) "output[" v:51 "]" " ←ᵢ " x:51 => MLIR.SetOutput v x
+
+end MLIRNotation
 
 abbrev MLIRProgram := MLIR NotInNondet
 
-open MLIR in
-lemma x : MLIRProgram := Sequence (Nondet (Assign "x" (Op.Isz ⟨"y"⟩))) (Assign "z" (Op.Const 4))
+-- open MLIR in
+-- lemma x : MLIRProgram := Sequence (Nondet (Assign "x" (Op.Isz ⟨"y"⟩))) (Assign "z" (Op.Const 4))
 
-open MLIR in
-lemma y : MLIR InNondet := Sequence ((Assign "x" (Op.Isz ⟨"y"⟩))) ((Assign "z" (Op.Const 4)))
-
-#check x
-#check y
-
--- -- Pure functional operations from the cirgen (circuit generation) MLIR dialect.
--- inductive Op where
---   | Const : Felt → Op
---   | True : Op
---   | GetInput : ℕ → Felt → Op
---   | GetOutput : ℕ → Felt → Op
---   | Sub : Variable Felt → Variable Felt → Op
---   | Mul : Variable Felt → Variable Felt → Op
---   | Isz : Variable Felt → Op
---   | Inv : Variable Felt → Op
---   | AndEqz : Variable Prop → Variable Felt → Op
---   | AndCond : Variable Prop → Variable Felt → Variable Prop → Op
+-- open MLIR in
+-- lemma y : MLIR InNondet := Sequence ((Assign "x" (Op.Isz ⟨"y"⟩))) ((Assign "z" (Op.Const 4)))
 
 namespace MLIRNotation
 
@@ -174,119 +210,74 @@ namespace MLIRNotation
 
 end MLIRNotation
 
--- Notation for Ops.
-namespace MLIRNotation
-
-scoped infix:55 " &₀ " => Op.AndEqz
-scoped notation:55 " guard " c " & " x " with " y:55 => Op.AndCond x c y
-scoped prefix:max "C" => Op.Const
-scoped notation:max "⊤" => Op.True
-scoped notation:max "input[" n "]" => Op.GetInput n 0
-scoped notation:max "output[" n "]" => Op.GetOutput n 0
-scoped prefix:57 "??₀" => Op.Isz
-scoped prefix:max "Inv" => Op.Inv
-
--- scoped prefix:max "C" => Op.Const
-
-
-end MLIRNotation
-
 -- instance : Inhabited Lit := ⟨(Lit.Val (-42))⟩
 
--- -- Evaluate a pure functional circuit operation to get some kind of literal.
--- def Op.eval (state : State) (op : Op) : Lit :=
---   match op with
---   | Const x => .Val x
---   | True => .Constraint (_root_.True)
---   | GetInput i _ => .Val <| state.input.getD i (-42)
---   | GetOutput i _ => .Val <| state.output.getD i (-42)
---   | Sub x y => .Val $ match state.felts x.name, state.felts y.name with
---                         | some x, some y => x - y
---                         | _      , _       => 42
---   | Mul x y => .Val $ match state.felts x.name, state.felts y.name with
---                         | some x, some y => x * y
---                         | _      , _       => 42
---   | AndEqz c x => .Constraint $ match state.props c.name, state.felts x.name with
---                     | some c, some x => c ∧ x = 0
---                     | _      , _     => 42 = 42
---   | AndCond old cond inner =>
---       .Constraint $ match state.props old.name, state.felts cond.name, state.props inner.name with
---         | .some old, .some cond, .some inner => if cond == 0 then old else old ∧ inner
---         | _        , _         , _           => 42 = 42
---   | Isz x => .Val $ match state.felts x.name with
---                | some x => if x == 0 then 1 else 0
---                | _      => 42
---   | Inv x => .Val $ match state.felts x.name with
---                | some x => if x == 0 then 0 else x⁻¹
---                | _      => 42
+namespace Op
 
--- namespace Op
+section Op
 
--- section Op
+open MLIRNotation
 
--- variable (state : State) (op : Op)
+variable (st : State) {α : IsNondet}
 
--- @[simp]
--- lemma eval_const {x : Felt} : Op.eval state (Const x) = .Val x := by rfl
+@[simp]
+lemma eval_const {x : Felt} : Γ st ⟦@Const α x⟧ₑ = .Val x := rfl
 
--- @[simp]
--- lemma eval_const_one : Op.eval state (Const 1 : Op) = .Val 1 := by rfl
+@[simp]
+lemma eval_true : Γ st ⟦@Op.True α⟧ₑ = .Constraint (_root_.True) := rfl
 
--- @[simp]
--- lemma eval_true : Op.eval state True = .Constraint (_root_.True) := by rfl
+@[simp]
+lemma eval_getInput {i : ℕ} {x : Felt} : Γ st ⟦@GetInput α i x⟧ₑ = .Val (st.input.getD i (-42)) := rfl
 
--- @[simp]
--- lemma eval_getInput {i : ℕ} {x : Felt} : Op.eval state (GetInput i x) = .Val (state.input.getD i (-42)) := by rfl
+@[simp]
+lemma eval_getOutput {i : ℕ} {x : Felt} : Γ st ⟦@GetOutput α i x⟧ₑ = .Val (st.output.getD i (-42)) := rfl
 
--- @[simp]
--- lemma eval_getOutput {i : ℕ} {x : Felt} : Op.eval state (GetOutput i x) = .Val (state.output.getD i (-42)) := by rfl
+@[simp]
+lemma eval_sub {x y : Variable Felt} :
+  Γ st ⟦@Sub α x y⟧ₑ = .Val (match st.felts x.name, st.felts y.name with
+                              | some x, some y => x - y
+                              | _      , _     => 42) := rfl
 
--- @[simp]
--- lemma eval_sub {x : Variable Felt} {y : Variable Felt} :
---   Op.eval state (Sub x y) = .Val (match state.felts x.name, state.felts y.name with
---                                       | some x, some y => x - y
---                                       | _      , _       => 42) := by rfl
- 
--- @[simp]
--- lemma eval_mul {x : Variable Felt} {y : Variable Felt} :
---   Op.eval state (Mul x y) = .Val (match state.felts x.name, state.felts y.name with
---                                       | some x, some y => x * y
---                                       | _      , _       => 42) := by rfl
+@[simp]
+lemma eval_mul {x y : Variable Felt} :
+  Γ st ⟦@Mul α x y⟧ₑ = .Val (match st.felts x.name, st.felts y.name with
+                              | some x, some y => x * y
+                              | _      , _     => 42) := rfl
 
--- @[simp]
--- lemma eval_isz {x : Variable Felt} :
---   Op.eval state (Isz x) = .Val (match state.felts x.name with
---                                   | some x => if x == 0 then 1 else 0
---                                   | _      => 42) := by rfl
--- @[simp]
--- lemma eval_inv {x : Variable Felt} :
---   Op.eval state (Inv x) = .Val (match state.felts x.name with
---                                   | some x => if x == 0 then 0 else x⁻¹
---                                   | _      => 42) := by rfl
+@[simp]
+lemma eval_isz {x : Variable Felt} :
+  Γ st ⟦??₀x⟧ₑ = .Val (match st.felts x.name with
+                        | some x => if x == 0 then 1 else 0
+                        | _      => 42) := rfl
+@[simp]
+lemma eval_inv {x : Variable Felt} :
+  Γ st ⟦Inv x⟧ₑ = .Val (match st.felts x.name with
+                         | some x => if x == 0 then 0 else x⁻¹
+                         | _      => 42) := rfl
 
--- -- lemma eval_eqz {c : Variable Prop}
--- --                {x : Variable Felt}
--- --     (h₁ : state.props c.name = some c₁)
--- --     (h₂ : state.felts x.name = some x₁) :
--- --   (AndEqz c x).eval state = .Constraint (c₁ ∧ x₁ = 0) := by simp [eval, *]
+-- lemma eval_eqz {c : Variable Prop}
+--                {x : Variable Felt}
+--     (h₁ : state.props c.name = some c₁)
+--     (h₂ : state.felts x.name = some x₁) :
+--   (AndEqz c x).eval state = .Constraint (c₁ ∧ x₁ = 0) := by simp [eval, *]
 
--- @[simp]
--- lemma eval_andEqz :
---   (AndEqz c x).eval state =
---     .Constraint (match state.props c.name, state.felts x.name with
---                  | some c, some x => (c ∧ x = 0)
---                  | _      , _     => (42 = 42)) := rfl
+@[simp]
+lemma eval_andEqz :
+  Γ st ⟦@AndEqz α c x⟧ₑ =
+    .Constraint (match st.props c.name, st.felts x.name with
+                   | some c, some x => (c ∧ x = 0)
+                   | _      , _     => (42 = 42)) := rfl
 
--- @[simp]
--- lemma eval_andCond :
---   (AndCond old cnd inner).eval state =
---     .Constraint (match state.props old.name, state.felts cnd.name, state.props inner.name with
---         | .some old, .some cnd, .some inner => if cnd == 0 then old else old ∧ inner
---         | _        , _         , _           => 42 = 42) := rfl
+@[simp]
+lemma eval_andCond :
+  Γ st ⟦@AndCond α old cnd inner⟧ₑ =
+    .Constraint (match st.props old.name, st.felts cnd.name, st.props inner.name with
+                  | .some old, .some cnd, .some inner => if cnd == 0 then old else old ∧ inner
+                  | _        , _         , _           => 42 = 42) := rfl
 
--- end Op
+end Op
 
--- end Op
+end Op
 
 -- -- Evaluate `op` and map `name ↦ result` in `state : State`.
 -- def Op.assign (state : State) (op : Op) (name : String) : State :=
